KoikaStd.v
@@ -1,0 +1,57 @@
+Require Import SGA.Notations.
+
+Definition pos_t := unit.
+Definition var_t := string.
+Definition fn_name_t := string.
+Notation uaction := (uaction pos_t var_t fn_name_t).
+Notation UInternalFunction reg_t ext_fn_t := (InternalFunction fn_name_t var_t (uaction reg_t ext_fn_t)).
+
+Module Type Fifo.
+  Parameter T:type.
+End Fifo.
+
+Module Fifo1 (f: Fifo).
+  Import f.
+  Inductive reg_t := data0 |  valid0.
+
+  Definition R r :=
+    match r with
+    | data0 => T
+    | valid0 => bits_t 1
+    end.
+
+  Notation zero := (Bits.zeroes _).
+
+  Definition r idx : R idx :=
+    match idx with
+    | data0 => value_of_bits zero
+    | valid0 => zero
+    end.
+
+  Definition name_reg r :=
+    match r with
+    | data0 => "data0"
+    | valid0 => "valid0"
+    end.
+
+
+  Definition enq : UInternalFunction reg_t empty_ext_fn_t :=
+    function (data : T) : bits_t 0 :=
+      if (!read0(valid0)) then
+        write0(data0,data);
+          write0(valid0,#Ob~1)
+      else
+        fail.
+
+
+  Definition deq :  UInternalFunction reg_t empty_ext_fn_t :=
+    function : T :=
+      if (read0(valid0)) then
+        write0(valid0,`UConstBits Ob~0`);
+          read0(data0)
+      else
+        fail(5).
+
+  Instance FiniteType_reg_t : FiniteType reg_t := _.
+
+End Fifo1.
